Jennisys/examples/mod2/jennisys-synth_List.dfy
@@ -37,12 +37,15 @@ class List<T> {
     ensures list[1] == q;
     ensures |list| == 2;
   {
-    var gensym68 := new Node<T>;
-    gensym68.Double(p, q);
+    var gensym78 := new Node<T>;
+    gensym78.Double(p, q);
     this.list := [p, q];
-    this.root := gensym68;
+    this.root := gensym78;
+
     // repr stuff
     this.Repr := {this} + this.root.Repr;
+    // assert repr objects are valid (helps verification)
+    assert gensym78.Valid();
   }
 
 
@@ -55,6 +58,7 @@ class List<T> {
   {
     this.list := [];
     this.root := null;
+
     // repr stuff
     this.Repr := {this};
   }
@@ -68,12 +72,15 @@ class List<T> {
     ensures list[0] == t;
     ensures |list| == 1;
   {
-    var gensym67 := new Node<T>;
-    gensym67.Init(t);
+    var gensym77 := new Node<T>;
+    gensym77.Init(t);
     this.list := [t];
-    this.root := gensym67;
+    this.root := gensym77;
+
     // repr stuff
     this.Repr := {this} + this.root.Repr;
+    // assert repr objects are valid (helps verification)
+    assert gensym77.Valid();
   }
 
 }
@@ -97,15 +104,17 @@ class Node<T> {
     reads *;
   {
     Valid_repr() &&
-    (next == null <==> (list == [data] && list[0] == data) && |list| == 1) &&
+    (next == null ==> (list == [data] && list[0] == data) && |list| == 1) &&
     (next != null ==> list == [data] + next.list) &&
     (|list| > 0)
   }
 
   function Valid(): bool
     reads *;
+    decreases Repr;
   {
     this.Valid_self() &&
+    (next != null ==> next.Valid()) &&
     (next != null ==> next.Valid_self()) &&
     (next != null && next.next != null ==> next.next.Valid_self())
   }
@@ -120,13 +129,58 @@ class Node<T> {
     ensures list[1] == q;
     ensures |list| == 2;
   {
-    var gensym74 := new Node<T>;
-    gensym74.Init(q);
+    var gensym87 := new Node<T>;
+    gensym87.Init(q);
     this.data := p;
     this.list := [p, q];
-    this.next := gensym74;
+    this.next := gensym87;
+
     // repr stuff
     this.Repr := {this} + this.next.Repr;
+    // assert repr objects are valid (helps verification)
+    assert gensym87.Valid();
+  }
+
+
+  method Find(n: T) returns (ret: bool)
+    requires Valid();
+    ensures fresh(Repr - old(Repr));
+    ensures Valid();
+    ensures ret == (n in list);
+    decreases Repr;
+  {
+    if (n != this.data && this.next == null) {
+      ret := n == this.data;
+    } else {
+      if (this.next != null) {
+        var x_6 := this.next.Find(n);
+        ret := n == this.data || x_6;
+      } else {
+        ret := true;
+      }
+    }
+  }
+
+
+  method Get(idx: int) returns (ret: T)
+    requires Valid();
+    requires idx >= 0;
+    requires idx < |list|;
+    ensures fresh(Repr - old(Repr));
+    ensures Valid();
+    ensures ret == list[idx];
+    decreases Repr;
+  {
+    if (this.next == null) {
+      ret := this.data;
+    } else {
+      if (idx == 0) {
+        ret := this.data;
+      } else {
+        var x_7 := this.next.Get(idx - 1);
+        ret := x_7;
+      }
+    }
   }
 
 
@@ -141,8 +195,53 @@ class Node<T> {
     this.data := t;
     this.list := [t];
     this.next := null;
+
     // repr stuff
     this.Repr := {this};
+  }
+
+
+  method List() returns (ret: seq<T>)
+    requires Valid();
+    ensures fresh(Repr - old(Repr));
+    ensures Valid();
+    ensures ret == list;
+    decreases Repr;
+  {
+    if (this.next == null) {
+      ret := [this.data];
+    } else {
+      var x_8 := this.next.List();
+      ret := [this.data] + x_8;
+    }
+  }
+
+
+  method Size() returns (ret: int)
+    requires Valid();
+    ensures fresh(Repr - old(Repr));
+    ensures Valid();
+    ensures ret == |list|;
+    decreases Repr;
+  {
+    if (this.next == null) {
+      ret := 1;
+    } else {
+      var x_9 := this.next.Size();
+      ret := 1 + x_9;
+    }
+  }
+
+
+  method Tail() returns (tail: Node<T>)
+    requires Valid();
+    ensures fresh(Repr - old(Repr));
+    ensures Valid();
+    ensures |list| == 1 ==> tail == null;
+    ensures |list| > 1 ==> tail != null && tail.list == list[1..];
+    ensures tail != null ==> tail.Valid();
+  {
+    tail := this.next;
   }
 
 }
